New file for codegen defs; refactor/clean up instrs

theories/compiler/instrs.v
@@ -19,517 +19,421 @@ From Wasm Require datatypes operations.
 Require Import Wasm.numerics.
 
 From RichWasm Require term typing.
-From RichWasm.compiler Require Import numerics types util.
+From RichWasm.compiler Require Import codegen numerics types util.
 Require Import RichWasm.util.dlist.
 Import RichWasm.util.dlist.Notation.
 
 Module R. Include term <+ typing. End R.
 Module W. Include datatypes <+ operations. End W.
 
-(* locals exclusive to webassembly (compiler-generated temporaries, etc) *)
-Notation wlocal_ctx := (list W.value_type) (only parsing).
-
-Notation dexpr := (dlist W.basic_instruction).
-
-Record codegen (A : Type) :=
-  { uncodegen : stateT wlocal_ctx
-                       (writerT (@DList.Monoid_dlist W.basic_instruction)
-                                (sum error))
-                       A }.
-
-Arguments Build_codegen {A} _.
-Arguments uncodegen {A} _.
-
-Existing Instance Monad_stateT.
-
-Global Instance Monad_codegen : Monad codegen :=
-  { ret := fun _ => Build_codegen ∘ ret;
-    bind := fun _ _ c f => Build_codegen (uncodegen c >>= uncodegen ∘ f) }.
-
-Global Instance MonadExc_codegen : MonadExc error codegen :=
-  { raise := fun _ => Build_codegen ∘ raise;
-    catch := fun _ b h => Build_codegen (catch (uncodegen b) (uncodegen ∘ h)) }.
-
-Global Instance MonadState_codegen : MonadState wlocal_ctx codegen :=
-  { get := Build_codegen get;
-    put := Build_codegen ∘ put }.
-
-Global Instance MonadWriter_codegen : MonadWriter (@DList.Monoid_dlist W.basic_instruction) codegen :=
-  { tell := Build_codegen ∘ tell;
-    listen := fun _ => Build_codegen ∘ listen ∘ uncodegen;
-    (* Work around broken implementation of `pass` in ExtLib.
-       https://github.com/rocq-community/coq-ext-lib/issues/153 *)
-    pass := fun _ c => Build_codegen (mkStateT (fun s =>
-      pass ('(x, f, s) <- runStateT (uncodegen c) s;;
-            ret (x, s, f)))) }.
-
-Definition lift_error {A} (c : error + A) : codegen A :=
-  Build_codegen (lift (lift c)).
-
-Definition try_option {A} (e : error) (x : option A) : codegen A :=
-  match x with
-  | None => raise e
-  | Some x' => ret x'
-  end.
-
-Definition run_codegen (c : codegen unit) (wl : wlocal_ctx) : error + wlocal_ctx * W.expr :=
-  match runWriterT (runStateT (uncodegen c) wl) with
-  | inl e => inl e
-  | inr x => inr (snd (PPair.pfst x), DList.to_list (PPair.psnd x))
-  end.
-
-Definition emit (e : W.basic_instruction) : codegen unit :=
-  tell (DList.singleton e).
-
-Definition capture {A} (c : codegen A) : codegen (A * dexpr) :=
-  censor (const []%DL) (listen c).
-
-Definition block_c {A} (tf : W.function_type) (c : codegen A) : codegen A :=
-  '(x, es) <- capture c;;
-  emit (W.BI_block tf (DList.to_list es));;
-  ret x.
-
-Definition loop_c {A} (tf : W.function_type) (c : codegen A) : codegen A :=
-  '(x, es) <- capture c;;
-  emit (W.BI_loop tf (DList.to_list es));;
-  ret x.
-
-Definition if_c {A B} (tf : W.function_type) (thn : codegen A) (els : codegen B) : codegen (A * B) :=
-  '(x1, es1) <- capture thn;;
-  '(x2, es2) <- capture els;;
-  emit (W.BI_if tf (DList.to_list es1) (DList.to_list es2));;
-  ret (x1, x2).
-
-Definition if_gc_bit_set {A B} (tf : W.function_type) (gc : codegen B) (mm : codegen A)
-  : codegen (A * B) :=
-  emit (W.BI_const (W.VAL_int32 (Wasm_int.int_of_Z numerics.i32m 1%Z)));;
-  emit (W.BI_binop W.T_i32 (W.Binop_i W.BOI_and));;
-  emit (W.BI_testop W.T_i32 W.TO_eqz);;
-  if_c tf mm gc.
-
-Definition unset_gc_bit : codegen unit :=
-  emit (W.BI_const (W.VAL_int32 (Wasm_int.int_of_Z numerics.i32m 1%Z)));;
-  emit (W.BI_binop W.T_i32 (W.Binop_i W.BOI_sub)).
-
-Fixpoint loads'
-  (mem : W.memidx)
-  (base_ptr_var : W.localidx)
-  (off : W.static_offset)
-  (tys : list W.value_type)
-  : codegen unit :=
-  match tys with
-  | [] => ret tt
-  | ty :: tys =>
-      emit (W.BI_get_local (localimm base_ptr_var));;
-      emit (W.BI_load (memimm mem) ty None 0%N off);;
-      loads' mem base_ptr_var (off + N.of_nat (W.length_t ty))%N tys
-  end.
-
-Definition loads mem base_ptr_var tys : codegen unit :=
-  loads' mem base_ptr_var 0%N tys.
-
-Fixpoint loc_stores'
-  (base_ptr_var : W.localidx)
-  (mem : W.memidx)
-  (off : W.static_offset)
-  (val_var_tys : list (W.localidx * W.value_type))
-  : codegen unit :=
-  match val_var_tys with
-  | [] => ret tt
-  | (val_var, ty) :: val_var_tys =>
-      emit (W.BI_get_local (localimm base_ptr_var));;
-      emit (W.BI_get_local (localimm val_var));;
-      emit (W.BI_store (memimm mem) ty None 0%N off);;
-      loc_stores' base_ptr_var mem (off + N.of_nat (W.length_t ty))%N val_var_tys
-  end.
-
-Definition loc_stores base_ptr_var mem val_var_tys : codegen unit :=
-  loc_stores' base_ptr_var mem 0%N val_var_tys.
-
-Definition stores base_ptr_var mem (val_vars : list W.localidx) (tys : list W.value_type)
-  : codegen unit :=
-  loc_stores base_ptr_var mem (zip val_vars tys).
-
-Inductive VarScope :=
-  | VSGlobal
-  | VSLocal.
-
-Definition scope_get_set (scope : VarScope) :
-  (W.immediate -> W.basic_instruction) *
-  (W.immediate -> W.basic_instruction) :=
-  match scope with
-  | VSGlobal => (W.BI_get_global, W.BI_set_global)
-  | VSLocal => (W.BI_get_local, W.BI_set_local)
-  end.
-
-Definition for_gc_ref_vars (scope : VarScope) (vars : list W.immediate) (m : codegen unit) : codegen unit :=
-  iterM
-    (fun var =>
-       let '(get, set) := scope_get_set scope in
-       emit (get var);;
-       if_gc_bit_set (W.Tf [W.T_i32] [W.T_i32]) m (ret tt);;
-       emit (set var))
-    vars.
-
-Fixpoint global_layout (globs : list R.GlobalType) (idx : nat) : option (W.globalidx * R.Typ) :=
-  match globs, idx with
-  | [R.GT _ ty], 0 => Some (W.Mk_globalidx 0, ty)
-  | R.GT _ ty :: globs', S idx' => global_layout globs' (length (translate_type ty) + idx')
-  | _, _ => None
-  end.
-
 Section Instrs.
 
   Variable me : module_env.
   Variable fe : function_env.
 
-  Definition wnext : codegen W.localidx :=
-    temps <- get;;
-    ret (W.Mk_localidx (fe.(fe_wlocal_offset) + length temps)).
+  Definition wlalloc (ty : W.value_type) : codegen W.localidx :=
+    wl <- get;;
+    put (wl ++ [ty]);;
+    ret (W.Mk_localidx (fe.(fe_wlocal_offset) + length wl)).
 
-  Definition walloc (t : W.value_type) : codegen W.localidx :=
-    temps <- get;;
-    put (temps ++ [t]);;
-    ret (W.Mk_localidx (fe.(fe_wlocal_offset) + length temps)).
-
-  Definition wallocs (tys : list W.value_type) : codegen (list W.localidx) :=
-    mapT walloc tys.
-
-  Definition walloc_args (tys : list W.value_type) : codegen (list W.localidx) :=
-    vars <- wallocs tys;;
-    @forT list _ _ _ _ _ vars (fun var => emit (W.BI_set_local (localimm var)));;
-    ret vars.
-
-  Definition walloc_rvalue (ty : R.Typ) : codegen W.localidx :=
-    i <- wnext;;
-    forT (translate_type ty) walloc;;
-    ret i.
-
-  Definition walloc_rvalues (tys : list R.Typ) : codegen W.localidx :=
-    i <- wnext;;
-    forT tys walloc_rvalue;;
-    ret i.
-
-  Definition tagged_store
-    (base_ptr : W.localidx)
-    (arg_vars : list W.localidx)
-    (get_offset : codegen unit)
-    (ty : R.Typ)
-    : codegen unit :=
-    emit (W.BI_tee_local (localimm base_ptr));;
-    emit (W.BI_get_local (localimm base_ptr));;
-    let tys := translate_type ty in
-    if_gc_bit_set (W.Tf [] [])
-      (emit (W.BI_get_local (localimm base_ptr));;
-       unset_gc_bit;;
-       get_offset;;
-       emit (W.BI_set_local (localimm base_ptr));;
-       stores base_ptr me.(me_runtime).(mr_mem_gc) arg_vars tys)
-      (emit (W.BI_get_local (localimm base_ptr));;
-       get_offset;;
-       stores base_ptr me.(me_runtime).(mr_mem_mm) arg_vars tys);;
-    ret tt.
-
-  Definition local_layout (L : R.Local_Ctx) (idx : nat) : error + (W.localidx * R.Typ) :=
-    let fix go L base i :=
-      match L, i with
-      | (τ, sz) :: L, 0 => inr (W.Mk_localidx base, τ)
-      | (τ, sz) :: L, S i =>
-          sz_const <- size_upper_bound fe.(fe_size_bounds) sz;;
-          go L (base + sz_const) i
-      | [], _ => inl (EIndexOutOfBounds idx)
-      end
-    in
-    go L 0 idx.
-
-  Definition gc_loads
-    (ref_var : W.localidx)
-    (get_offset : codegen unit)
-    (tys : list W.value_type)
-    : codegen unit :=
-    base_ptr_var <- walloc W.T_i32;;
-    emit (W.BI_get_local (localimm ref_var));;
-    unset_gc_bit;;
-    get_offset;;
-    emit (W.BI_binop W.T_i32 (W.Binop_i W.BOI_add));;
-    emit (W.BI_set_local (localimm base_ptr_var));;
-    loads me.(me_runtime).(mr_mem_gc) base_ptr_var tys.
-
-  Definition lin_loads
-    (ref_var : W.localidx)
-    (get_offset : codegen unit)
-    (tys : list W.value_type)
-    : codegen unit :=
-    base_ptr_var <- walloc W.T_i32;;
-    emit (W.BI_get_local (localimm ref_var));;
-    get_offset;;
-    emit (W.BI_binop W.T_i32 (W.Binop_i W.BOI_add));;
-    emit (W.BI_set_local (localimm base_ptr_var));;
-    loads me.(me_runtime).(mr_mem_mm) base_ptr_var tys.
-
-  Definition tagged_loads
-    (base_ptr: W.localidx)
-    (get_offset: codegen unit)
-    (tys: list W.value_type)
-    : codegen unit :=
-    emit (W.BI_get_local (localimm base_ptr));;
-    if_gc_bit_set (W.Tf [] tys)
-      (gc_loads base_ptr get_offset tys)
-      (lin_loads base_ptr get_offset tys);;
-    ret tt.
-
-  Definition tagged_load
-    (base_ptr : W.localidx)
-    (get_offset : codegen unit)
-    (ty : R.Typ)
-    : codegen unit :=
-    let tys := translate_type ty in
-    tagged_loads base_ptr get_offset tys.
-
-  Definition tagged_store' (get_offset : codegen unit) (ty : R.Typ) : codegen unit :=
-    let tys := translate_type ty in
-    arg_vars <- walloc_args tys;;
-    base_ptr_var <- walloc W.T_i32;;
-    tagged_store base_ptr_var arg_vars get_offset ty.
-
-  Definition get_i64_local (loc : W.localidx) : codegen unit :=
-    emit (W.BI_get_local (localimm loc));;
+  Definition get_local_i64 (x : W.localidx) : codegen unit :=
+    emit (W.BI_get_local (localimm x));;
     emit (W.BI_cvtop W.T_i32 W.CVO_reinterpret W.T_i64 None);;
-    emit (W.BI_get_local (localimm loc + 1));;
+    emit (W.BI_get_local (localimm x + 1));;
     emit (W.BI_const (W.VAL_int64 (Wasm_int.int_of_Z i64m 32)));;
     emit (W.BI_binop W.T_i64 (W.Binop_i W.BOI_rotl));;
     emit (W.BI_cvtop W.T_i32 W.CVO_reinterpret W.T_i64 None);;
     emit (W.BI_binop W.T_i64 (W.Binop_i W.BOI_or)).
 
-  Definition set_i64_local (loc : W.localidx) : codegen unit :=
-    tmp <- walloc W.T_i64;;
-    emit (W.BI_tee_local (localimm tmp));;
+  Definition set_local_i64 (x : W.localidx) : codegen unit :=
+    y <- wlalloc W.T_i64;;
+    emit (W.BI_tee_local (localimm y));;
     emit (W.BI_const (W.VAL_int64 (wasm_extend_u int32_minus_one)));;
     emit (W.BI_binop W.T_i64 (W.Binop_i W.BOI_and));;
     emit (W.BI_cvtop W.T_i64 W.CVO_convert W.T_i32 None);;
-    emit (W.BI_set_local (localimm loc));;
-    emit (W.BI_get_local (localimm tmp));;
+    emit (W.BI_set_local (localimm x));;
+    emit (W.BI_get_local (localimm y));;
     emit (W.BI_const (W.VAL_int64 (Wasm_int.int_of_Z i64m 32)));;
     emit (W.BI_binop W.T_i64 (W.Binop_i W.BOI_rotr));;
-    emit (W.BI_set_local (localimm loc + 1)).
+    emit (W.BI_set_local (localimm x + 1)).
 
-  Definition numtyp_gets (ty : R.NumType) (loc : W.localidx) : codegen unit :=
+  Definition get_local_w (x : W.localidx) (ty : W.value_type) : codegen unit :=
     match ty with
-    | R.Int s R.i32 => emit (W.BI_get_local (localimm loc))
-    | R.Float R.f32 =>
-        emit (W.BI_get_local (localimm loc));;
+    | W.T_i32 => emit (W.BI_get_local (localimm x))
+    | W.T_i64 => get_local_i64 x
+    | W.T_f32 =>
+        emit (W.BI_get_local (localimm x));;
         emit (W.BI_cvtop W.T_i32 W.CVO_reinterpret W.T_f32 None)
-    | R.Int s R.i64 => get_i64_local loc
-    | R.Float R.f64 =>
-        get_i64_local loc;;
+    | W.T_f64 =>
+        get_local_i64 x;;
         emit (W.BI_cvtop W.T_i64 W.CVO_reinterpret W.T_f64 None)
     end.
 
-  Definition numtyp_sets (ty : R.NumType) (loc : W.localidx) : codegen unit :=
+  Definition get_locals_w (x : W.localidx) : W.result_type -> codegen unit :=
+    ignore ∘ foldM
+      (fun ty x =>
+        get_local_w (W.Mk_localidx x) ty;;
+        ret (x + W.words_t ty))
+      (ret (localimm x)).
+
+  Definition set_local_w (x : W.localidx) (ty : W.value_type) : codegen unit :=
     match ty with
-    | R.Int s R.i32 => emit (W.BI_set_local (localimm loc))
-    | R.Float R.f32 =>
+    | W.T_i32 => emit (W.BI_set_local (localimm x))
+    | W.T_i64 => set_local_i64 x
+    | W.T_f32 =>
         emit (W.BI_cvtop W.T_f32 W.CVO_reinterpret W.T_i32 None);;
-        emit (W.BI_set_local (localimm loc))
-    | R.Int s R.i64 => set_i64_local loc
-    | R.Float R.f64 =>
+        emit (W.BI_set_local (localimm x))
+    | W.T_f64 =>
         emit (W.BI_cvtop W.T_f64 W.CVO_reinterpret W.T_i64 None);;
-        set_i64_local loc
+        set_local_i64 x
     end.
 
-  Fixpoint local_gets (ty : R.Typ) (loc : W.localidx) : codegen unit :=
-    match ty with
-    | R.Num nτ => numtyp_gets nτ loc
-    | R.TVar α => emit (W.BI_get_local (localimm loc))
-    | R.Unit => ret tt
-    | R.ProdT τs =>
-        let fix loop τs0 sz :=
-          match τs0 with
-          | τ0 :: τs0' =>
-              let sz := type_words τ0 in
-              local_gets τ0 loc;;
-              loop τs0' (localimm loc + sz)
-          | [] => ret tt
-          end in
-        loop τs (localimm loc)
-    | R.CoderefT χ => emit (W.BI_get_local (localimm loc))
-    | R.Rec q τ => local_gets τ loc
-    | R.PtrT ℓ => emit (W.BI_get_local (localimm loc))
-    | R.ExLoc q τ => local_gets τ loc
-    | R.OwnR ℓ => ret tt
-    | R.CapT cap ℓ ψ => ret tt
-    | R.RefT cap ℓ ψ => emit (W.BI_get_local (localimm loc))
-    end.
+  Definition set_locals_w (x : W.localidx) : W.result_type -> codegen unit :=
+    ignore ∘ foldM
+      (fun ty x =>
+        set_local_w (W.Mk_localidx x) ty;;
+        ret (x + W.words_t ty))
+      (ret (localimm x)).
 
-  Fixpoint local_sets (ty : R.Typ) (loc : W.localidx) : codegen unit :=
-    match ty with
-    | R.Num nτ =>
-        numtyp_sets nτ loc
-    | R.TVar α =>
-        emit (W.BI_set_local (localimm loc))
-    | R.Unit =>
-        ret tt
-    | R.ProdT τs =>
-        let fix loop τs0 sz :=
-          match τs0 with
-          | τ0 :: τs0' =>
-              let sz := type_words τ0 in
-              local_sets τ0 loc;;
-              loop τs0' (localimm loc + sz)
-          | [] => ret tt
-          end in
-        loop τs (localimm loc)
-    | R.CoderefT χ =>
-        emit (W.BI_set_local (localimm loc))
-    | R.Rec q τ =>
-        local_sets τ loc
-    | R.PtrT ℓ =>
-        emit (W.BI_set_local (localimm loc))
-    | R.ExLoc q τ =>
-        local_sets τ loc
-    | R.OwnR ℓ =>
-        ret tt
-    | R.CapT cap ℓ ψ =>
-        ret tt
-    | R.RefT cap ℓ ψ =>
-        emit (W.BI_set_local (localimm loc))
-    end.
+  Definition get_local (x : W.localidx) : R.Typ -> codegen unit :=
+    get_locals_w x ∘ translate_type.
 
-  Definition save_stack (tys : list R.Typ) : codegen W.localidx :=
-    idx <- walloc_rvalues tys;;
-    local_sets (R.ProdT tys) idx;;
-    ret idx.
+  Definition set_local (x : W.localidx) : R.Typ -> codegen unit :=
+    set_locals_w x ∘ translate_type.
 
-  Definition restore_stack (tys : list R.Typ) (idx : W.localidx) : codegen unit :=
-    local_gets (R.ProdT tys) idx.
+  Definition save_stack_w (ty : W.result_type) : codegen W.localidx :=
+    xs <- forT ty wlalloc;;
+    ret (ssrfun.Option.default (W.Mk_localidx 0) (head xs)).
 
-  Fixpoint compile_sz (sz : R.Size) : codegen unit :=
+  Definition save_stack : list R.Typ -> codegen W.localidx :=
+    save_stack_w ∘ flat_map translate_type.
+
+  Definition restore_stack_w (x : W.localidx) (ty : W.result_type) : codegen unit :=
+    ignore (forT (seq (localimm x) (length ty)) (emit ∘ W.BI_get_local)).
+
+  Definition restore_stack (x : W.localidx) : list R.Typ -> codegen unit :=
+    restore_stack_w x ∘ flat_map translate_type.
+
+  Definition if_gc_bit {A B} (tf : W.function_type) (gc : codegen B) (mm : codegen A) : codegen (A * B) :=
+    emit (W.BI_const (W.VAL_int32 (Wasm_int.int_of_Z numerics.i32m 1%Z)));;
+    emit (W.BI_binop W.T_i32 (W.Binop_i W.BOI_and));;
+    emit (W.BI_testop W.T_i32 W.TO_eqz);;
+    if_c tf mm gc.
+
+  Definition clear_gc_bit : codegen unit :=
+    emit (W.BI_const (W.VAL_int32 (Wasm_int.int_of_Z numerics.i32m 1%Z)));;
+    emit (W.BI_binop W.T_i32 (W.Binop_i W.BOI_sub)).
+
+  Definition load_values_w (mem : W.memidx) (ptr : W.localidx) (off : W.static_offset)
+    : W.result_type -> codegen unit :=
+    ignore ∘ foldM
+      (fun ty off =>
+        emit (W.BI_get_local (localimm ptr));;
+        emit (W.BI_load (memimm mem) ty None 0%N off);;
+        ret (off + N.of_nat (W.length_t ty))%N)
+      (ret off).
+
+  Definition load_value (mem : W.memidx) (ptr : W.localidx) (off : W.static_offset)
+    : R.Typ -> codegen unit :=
+    load_values_w mem ptr off ∘ translate_type.
+
+  Definition load_value_tagged_w (get_offset : codegen unit) (ty : W.value_type) : codegen unit :=
+    ptr <- wlalloc W.T_i32;;
+    emit (W.BI_tee_local (localimm ptr));;
+    emit (W.BI_get_local (localimm ptr));;
+    if_gc_bit (W.Tf [] [])
+      (clear_gc_bit;;
+       get_offset;;
+       emit (W.BI_binop W.T_i32 (W.Binop_i W.BOI_add));;
+       emit (W.BI_load (memimm me.(me_runtime).(mr_mem_gc)) ty None 0%N 0%N))
+      (get_offset;;
+       emit (W.BI_binop W.T_i32 (W.Binop_i W.BOI_add));;
+       emit (W.BI_load (memimm me.(me_runtime).(mr_mem_mm)) ty None 0%N 0%N));;
+    ret tt.
+
+  Definition set_offset (ptr : W.localidx) (get_offset : codegen unit) : codegen unit :=
+    get_offset;;
+    emit (W.BI_binop W.T_i32 (W.Binop_i W.BOI_add));;
+    emit (W.BI_set_local (localimm ptr)).
+
+  Definition load_value_tagged (get_offset : codegen unit) (ty : R.Typ) : codegen unit :=
+    ptr <- wlalloc W.T_i32;;
+    emit (W.BI_tee_local (localimm ptr));;
+    emit (W.BI_get_local (localimm ptr));;
+    if_gc_bit (W.Tf [] [])
+      (clear_gc_bit;;
+       set_offset ptr get_offset;;
+       load_value me.(me_runtime).(mr_mem_gc) ptr 0%N ty)
+      (set_offset ptr get_offset;;
+       load_value me.(me_runtime).(mr_mem_mm) ptr 0%N ty);;
+    ret tt.
+
+  Definition store_value_w
+    (mem : W.memidx) (ptr : W.localidx) (off : W.static_offset)
+    (val : W.localidx) (ty : W.value_type)
+    : codegen unit :=
+    emit (W.BI_get_local (localimm ptr));;
+    emit (W.BI_get_local (localimm val));;
+    emit (W.BI_store (memimm mem) ty None 0%N off).
+
+  Definition store_values_w (mem : W.memidx) (ptr : W.localidx) (off : W.static_offset)
+    : list (W.localidx * W.value_type) -> codegen unit :=
+    ignore ∘ foldM
+      (fun '(val, ty) off =>
+        store_value_w mem ptr off val ty;;
+        ret (off + N.of_nat (W.length_t ty))%N)
+      (ret off).
+
+  Definition store_value (mem : W.memidx) (ptr : W.localidx) (off : W.static_offset) (val : W.localidx) (ty : R.Typ)
+    : codegen unit :=
+    let ty' := translate_type ty in
+    let vals := zip (map W.Mk_localidx (seq (localimm val) (length ty'))) ty' in
+    store_values_w mem ptr off vals.
+
+  Definition store_value_tagged (get_offset : codegen unit) (ty : R.Typ) : codegen unit :=
+    val <- save_stack [ty];;
+    ptr <- wlalloc W.T_i32;;
+    emit (W.BI_tee_local (localimm ptr));;
+    emit (W.BI_get_local (localimm ptr));;
+    if_gc_bit (W.Tf [] [])
+      (clear_gc_bit;;
+       set_offset ptr get_offset;;
+       store_value me.(me_runtime).(mr_mem_gc) ptr 0%N val ty)
+      (set_offset ptr get_offset;;
+       store_value me.(me_runtime).(mr_mem_mm) ptr 0%N val ty);;
+    ret tt.
+
+  Definition foreach_if_gc_bit (scope : VarScope) (refs : list W.immediate) (c : codegen unit)
+    : codegen unit :=
+    iterM
+      (fun var =>
+        let '(get, set) := scope_get_set scope in
+        emit (get var);;
+        if_gc_bit (W.Tf [W.T_i32] [W.T_i32]) c (ret tt);;
+        emit (set var))
+      refs.
+
+  Definition lookup_local (L : R.Local_Ctx) (idx : nat) : error + (W.localidx * R.Typ) :=
+    let fix go L i j :=
+      match L, j with
+      | (ty, sz) :: _, 0 => inr (W.Mk_localidx i, ty)
+      | (ty, sz) :: L', S j' =>
+          real_sz <- size_upper_bound fe.(fe_size_bounds) sz;;
+          go L' (i + real_sz) j'
+      | [], _ => inl (EIndexOutOfBounds idx)
+      end
+    in
+    go L 0 idx.
+
+  Definition lookup_global (idx : nat) : option (W.globalidx * R.Typ) :=
+    let fix go globals idx :=
+      match globals, idx with
+      | R.GT _ ty :: _, 0 => Some (W.Mk_globalidx 0, ty)
+      | R.GT _ ty :: globals', S idx' =>
+          let width := length (translate_type ty) in
+          go globals' (width + idx')
+      | [], _ => None
+      end
+    in
+    go me.(me_globals) idx.
+
+  Fixpoint compile_size (sz : R.Size) : codegen unit :=
     match sz with
     | R.SizeVar σ =>
-      local_idx <- try_option (EIndexOutOfBounds σ) (lookup σ fe.(fe_size_locals));;
-      emit (W.BI_get_local (localimm local_idx))
+        x <- try_option (EIndexOutOfBounds σ) (lookup σ fe.(fe_size_locals));;
+        emit (W.BI_get_local (localimm x))
     | R.SizePlus sz1 sz2 =>
-      compile_sz sz1;;
-      compile_sz sz2;;
-      emit (W.BI_binop W.T_i32 (W.Binop_i W.BOI_add))
+        compile_size sz1;;
+        compile_size sz2;;
+        emit (W.BI_binop W.T_i32 (W.Binop_i W.BOI_add))
     | R.SizeConst c =>
-      emit (W.BI_const (W.VAL_int32 (Wasm_int.int_of_Z i32m (Z.of_nat c))))
+        emit (W.BI_const (W.VAL_int32 (Wasm_int.int_of_Z i32m (Z.of_nat c))))
     end.
 
-  Definition compile_ind (ind: R.Index) : codegen unit :=
-    match ind with
-    | R.SizeI sz => compile_sz sz
+  Definition compile_index (idx: R.Index) : codegen unit :=
+    match idx with
+    | R.SizeI sz => compile_size sz
     | R.LocI _
     | R.QualI _
     | R.TypI _ => ret tt
     end.
 
-  Definition array_bounds_check (base idx : W.localidx) : codegen unit :=
-    tagged_load
-      base
+  Definition if_index_in_bounds {A} (tf : W.function_type) (idx : W.localidx) (c : codegen A)
+    : codegen A :=
+    load_value_tagged_w
       (emit (W.BI_const (W.VAL_int32 (Wasm_int.int_of_Z i32m (Z.of_nat 0)))))
-      (R.Num (R.Int R.U R.i32));;
+      (W.T_i32);;
     emit (W.BI_get_local (localimm idx));;
-    emit (W.BI_relop W.T_i32 (W.Relop_i (W.ROI_lt (W.SX_U)))).
+    emit (W.BI_relop W.T_i32 (W.Relop_i (W.ROI_lt (W.SX_U))));;
+    fst <$> if_c tf c (emit W.BI_unreachable).
 
-  Definition array_offset (idx : W.localidx) (size : nat) : codegen unit :=
+  Definition get_elem_offset (idx : W.localidx) (size : nat) : codegen unit :=
     emit (W.BI_get_local (localimm idx));;
     emit (W.BI_const (W.VAL_int32 (Wasm_int.int_of_Z i32m (Z.of_nat size))));;
     emit (W.BI_binop W.T_i32 (W.Binop_i W.BOI_mul));;
-    emit (W.BI_const (W.VAL_int32 (Wasm_int.int_of_Z i32m (Z.of_nat 4))));; (* skip header length word *)
+    (* Skip 4 bytes for the array length. *)
+    emit (W.BI_const (W.VAL_int32 (Wasm_int.int_of_Z i32m (Z.of_nat 4))));;
     emit (W.BI_binop W.T_i32 (W.Binop_i W.BOI_add)).
+
+  Definition compile_drop (ty : R.Typ) : codegen unit :=
+    val <- save_stack [ty];;
+    let refs := map (fun i => localimm val + i) (find_refs LMNative ty) in
+    foreach_if_gc_bit VSLocal refs
+      (emit (W.BI_call (funcimm me.(me_runtime).(mr_func_unregisterroot))));;
+    restore_stack val [ty];;
+    let tys := translate_type ty in
+    forT tys (const (emit W.BI_drop));;
+    ret tt.
+
+  Definition compile_return (ty : list R.Typ) : codegen unit :=
+    let return_ty := ssrfun.Option.default [] fe.(fe_return_type) in
+    let drop_ty := take (length ty - length return_ty) ty in
+    r <- save_stack return_ty;;
+    d <- save_stack drop_ty;;
+    let refs := map (fun i => localimm d + i) (flat_map (find_refs LMNative) drop_ty) in
+    foreach_if_gc_bit VSLocal refs
+      (emit (W.BI_call (funcimm me.(me_runtime).(mr_func_unregisterroot))));;
+    restore_stack r return_ty;;
+    emit W.BI_return.
+
+  Definition compile_get_local (L : R.Local_Ctx) (x : nat) : codegen unit :=
+    '(x', ty) <- lift_error (lookup_local L x);;
+    get_local x' ty;;
+    val <- save_stack [ty];;
+    let refs := map (fun i => localimm val + i) (find_refs LMNative ty) in
+    foreach_if_gc_bit VSLocal refs
+      (emit (W.BI_call (funcimm me.(me_runtime).(mr_func_duproot))));;
+    restore_stack val [ty].
+
+  Definition compile_set_local (L : R.Local_Ctx) (x : nat) : codegen unit :=
+    '(x', ty) <- lift_error (lookup_local L x);;
+    let refs := map (fun i => localimm x' + i) (find_refs LMWords ty) in
+    foreach_if_gc_bit VSLocal refs
+      (emit (W.BI_call (funcimm me.(me_runtime).(mr_func_unregisterroot))));;
+    set_local x' ty.
+
+  Definition compile_get_global (x : nat) : codegen unit :=
+    '(x', ty) <- try_option (EIndexOutOfBounds x) (lookup_global x);;
+    forT (imap (fun i _ => globalimm x' + i) (translate_type ty))
+      (emit ∘ W.BI_get_global);;
+    val <- save_stack [ty];;
+    let refs := map (fun i => localimm val + i) (find_refs LMNative ty) in
+    foreach_if_gc_bit VSLocal refs
+      (emit (W.BI_call (funcimm me.(me_runtime).(mr_func_duproot))));;
+    restore_stack val [ty].
+
+  Definition compile_set_global (x : nat) : codegen unit :=
+    '(x', ty) <- try_option (EIndexOutOfBounds x) (lookup_global x);;
+    let refs := map (fun i => globalimm x' + i) (find_refs LMNative ty) in
+    foreach_if_gc_bit VSGlobal refs
+      (emit (W.BI_call (funcimm me.(me_runtime).(mr_func_unregisterroot))));;
+    forT (imap (fun i _ => globalimm x' + i) (translate_type ty))
+      (emit ∘ W.BI_set_global);;
+    ret tt.
+
+  Definition compile_coderef (x : nat) : codegen unit :=
+    emit (W.BI_const (W.VAL_int32 (Wasm_int.int_of_Z i32m (Z.of_nat x))));;
+    emit (W.BI_get_global (globalimm me.(me_runtime).(mr_global_table_offset)));;
+    emit (W.BI_binop W.T_i32 (W.Binop_i W.BOI_add)).
+
+  Definition compile_call_indirect (arg_ty : list R.Typ) (idxs : list R.Index) : codegen unit :=
+    arg <- save_stack arg_ty;;
+    forT idxs compile_index;;
+    restore_stack arg arg_ty;;
+    emit (W.BI_call_indirect (tableimm me.(me_runtime).(mr_table))).
+
+  Definition compile_call (arg_ty : list R.Typ) (x : nat) (idxs : list R.Index) : codegen unit :=
+    arg <- save_stack arg_ty;;
+    forT idxs compile_index;;
+    restore_stack arg arg_ty;;
+    (* TODO: Translate function index. *)
+    emit (W.BI_call x).
+
+  Definition compile_struct_get (fields : list (R.Typ * R.Size)) (i : nat) : codegen unit :=
+    field_ty <- try_option EWrongTypeAnn (fst <$> lookup i fields);;
+    offset <- lift_error (struct_field_offset fields i);;
+    ref <- wlalloc W.T_i32;;
+    load_value_tagged (compile_size offset) field_ty;;
+    val <- save_stack [field_ty];;
+    let refs := map (fun i => localimm val + i) (find_refs LMNative field_ty) in
+    emit (W.BI_get_local (localimm ref));;
+    if_gc_bit (W.Tf [] [])
+      (foreach_if_gc_bit VSLocal refs
+         (emit (W.BI_call (funcimm me.(me_runtime).(mr_func_registerroot)))))
+      (foreach_if_gc_bit VSLocal refs
+         (emit (W.BI_call (funcimm me.(me_runtime).(mr_func_duproot)))));;
+    restore_stack val [field_ty].
+
+  Definition compile_struct_set (fields : list (R.Typ * R.Size)) (val_ty : R.Typ) (i : nat) : codegen unit :=
+    field_ty <- try_option EWrongTypeAnn (fst <$> lookup i fields);;
+    offset <- lift_error (struct_field_offset fields i);;
+
+    val <- save_stack [val_ty];;
+    ptr <- wlalloc W.T_i32;;
+    emit (W.BI_tee_local (localimm ptr));;
+    if_gc_bit (W.Tf [] [])
+      (let refs := map (fun i => localimm val + i) (find_refs LMNative val_ty) in
+       foreach_if_gc_bit VSLocal refs
+         (emit (W.BI_call (funcimm me.(me_runtime).(mr_func_unregisterroot)))))
+      (emit (W.BI_get_local (localimm ptr));;
+       ptr' <- wlalloc W.T_i32;;
+       set_offset ptr' (compile_size offset);;
+       load_value me.(me_runtime).(mr_mem_mm) ptr' 0%N field_ty;;
+       old_val <- save_stack [field_ty];;
+       let refs := map (fun i => localimm val + i) (find_refs LMNative field_ty) in
+       foreach_if_gc_bit VSLocal refs
+         (emit (W.BI_call (funcimm me.(me_runtime).(mr_func_unregisterroot)))));;
+
+    emit (W.BI_get_local (localimm ptr));;
+    store_value_tagged (compile_size offset) val_ty.
+
+  Definition compile_array_get (elem_ty : R.Typ) : codegen unit :=
+    (* TODO: registerroot if GC array; duproot if MM array. *)
+    idx <- wlalloc W.T_i32;;
+    ptr <- wlalloc W.T_i32;;
+    emit (W.BI_set_local (localimm idx));;
+    emit (W.BI_tee_local (localimm ptr));;
+    let elem_tys := translate_type elem_ty in
+    if_index_in_bounds (W.Tf [] elem_tys) idx
+      (emit (W.BI_get_local (localimm ptr));;
+       load_value_tagged (get_elem_offset idx (type_words elem_ty)) elem_ty).
+
+  Definition compile_array_set (elem_ty : R.Typ) : codegen unit :=
+    (* TODO: unregisterroot if GC array; duproot a bunch of times if MM array. *)
+    val <- save_stack [elem_ty];;
+    idx <- wlalloc W.T_i32;;
+    ptr <- wlalloc W.T_i32;;
+    emit (W.BI_set_local (localimm idx));;
+    emit (W.BI_tee_local (localimm ptr));;
+    if_index_in_bounds (W.Tf [] []) idx
+      (emit (W.BI_get_local (localimm ptr));;
+       restore_stack val [elem_ty];;
+       store_value_tagged (get_elem_offset idx (type_words elem_ty)) elem_ty).
 
   Fixpoint compile_instr (e : R.instr R.TyAnn) : codegen unit :=
     match e with
-    | R.INumConst _ ty n =>
-        let ty' := translate_num_type ty in
-        emit (W.BI_const (compile_Z ty' (Z.of_nat n)))
+    | R.INumConst _ ty n => emit (W.BI_const (compile_Z (translate_num_type ty) (Z.of_nat n)))
     | R.IUnit _ => ret tt
     | R.INum _ e' => emit (compile_num_instr e')
     | R.IUnreachable _ => emit (W.BI_unreachable)
     | R.INop _ => emit W.BI_nop
-    | R.IDrop (R.Arrow in_ty _, _) =>
-        ty <- try_option EWrongTypeAnn (head in_ty);;
-        let tys := translate_type ty in
-        val <- save_stack [ty];;
-        let refs := map (fun i => localimm val + i) (find_refs LMNative ty) in
-        for_gc_ref_vars VSLocal refs
-          (emit (W.BI_call (funcimm me.(me_runtime).(mr_func_unregisterroot))));;
-        restore_stack [ty] val;;
-        forT tys (const (emit W.BI_drop));;
-        ret tt
-    | R.IBlock _ ty _ es =>
-        block_c (translate_arrow_type ty) (forT es compile_instr);;
-        ret tt
-    | R.ILoop _ ty es =>
-        loop_c (translate_arrow_type ty) (forT es compile_instr);;
-        ret tt
+    | R.IDrop (R.Arrow ty _, _) => try_option EWrongTypeAnn (head ty) >>= compile_drop
+    | R.IBlock _ ty _ es => ignore (block_c (translate_arrow_type ty) (forT es compile_instr))
+    | R.ILoop _ ty es => ignore (loop_c (translate_arrow_type ty) (forT es compile_instr))
     | R.IIte _ ty _ es1 es2 =>
-        let ty' := translate_arrow_type ty in
-        if_c ty' (forT es1 compile_instr) (forT es2 compile_instr);;
-        ret tt
+        ignore (if_c (translate_arrow_type ty) (forT es1 compile_instr) (forT es2 compile_instr))
     | R.IBr _ l => emit (W.BI_br l)
     | R.IBrIf _ l => emit (W.BI_br_if l)
     | R.IBrTable _ ls l => emit (W.BI_br_table ls l)
-    | R.IRet (R.Arrow in_ty _, _) =>
-        let return_ty := ssrfun.Option.default [] fe.(fe_return_type) in
-        let drop_ty := take (length in_ty - length return_ty) in_ty in
-        r <- save_stack return_ty;;
-        d <- save_stack drop_ty;;
-        let refs := map (fun i => localimm d + i) (flat_map (find_refs LMNative) drop_ty) in
-        for_gc_ref_vars VSLocal refs
-          (emit (W.BI_call (funcimm me.(me_runtime).(mr_func_unregisterroot))));;
-        restore_stack return_ty r;;
-        emit W.BI_return
-    | R.IGetLocal (_, R.LSig L _) x _ =>
-        '(x', ty) <- lift_error (local_layout L x);;
-        local_gets ty x';;
-        val <- save_stack [ty];;
-        let refs := map (fun i => localimm val + i) (find_refs LMNative ty) in
-        for_gc_ref_vars VSLocal refs
-          (emit (W.BI_call (funcimm me.(me_runtime).(mr_func_duproot))));;
-        restore_stack [ty] val
-    | R.ISetLocal (_, R.LSig L _) x =>
-        '(x', ty) <- lift_error (local_layout L x);;
-        let refs := map (fun i => localimm x' + i) (find_refs LMWords ty) in
-        for_gc_ref_vars VSLocal refs
-          (emit (W.BI_call (funcimm me.(me_runtime).(mr_func_unregisterroot))));;
-        local_sets ty x'
-    | R.IGetGlobal _ x =>
-        '(x', ty) <- try_option (EIndexOutOfBounds x) (global_layout me.(me_globals) x);;
-        forT (imap (fun i _ => globalimm x' + i) (translate_type ty))
-          (emit ∘ W.BI_get_global);;
-        val <- save_stack [ty];;
-        let refs := map (fun i => localimm val + i) (find_refs LMNative ty) in
-        for_gc_ref_vars VSLocal refs
-          (emit (W.BI_call (funcimm me.(me_runtime).(mr_func_duproot))));;
-        restore_stack [ty] val
-    | R.ISetGlobal _ x =>
-        '(x', ty) <- try_option (EIndexOutOfBounds x) (global_layout me.(me_globals) x);;
-        let refs := map (fun i => globalimm x' + i) (find_refs LMNative ty) in
-        for_gc_ref_vars VSGlobal refs
-          (emit (W.BI_call (funcimm me.(me_runtime).(mr_func_unregisterroot))));;
-        forT (imap (fun i _ => globalimm x' + i) (translate_type ty))
-          (emit ∘ W.BI_set_global);;
-        ret tt
-    | R.ICoderef _ x =>
-        emit (W.BI_const (W.VAL_int32 (Wasm_int.int_of_Z i32m (Z.of_nat x))));;
-        emit (W.BI_get_global (globalimm me.(me_runtime).(mr_global_table_offset)));;
-        emit (W.BI_binop W.T_i32 (W.Binop_i W.BOI_add))
-    | R.ICallIndirect (R.Arrow in_ty _, _) idxs =>
-        args <- save_stack in_ty;;
-        forT idxs compile_ind;;
-        restore_stack in_ty args;;
-        emit (W.BI_call_indirect (tableimm me.(me_runtime).(mr_table)))
-    | R.ICall (R.Arrow in_ty _, _) x idxs =>
-        args <- save_stack in_ty;;
-        forT idxs compile_ind;;
-        restore_stack in_ty args;;
-        (* TODO: Translate function index. *)
-        emit (W.BI_call x)
-    | R.IMemUnpack _ ty _ es =>
-        block_c (translate_arrow_type ty) (forT es compile_instr);;
-        ret tt
+    | R.IRet (R.Arrow ty _, _) => compile_return ty
+    | R.IGetLocal (_, R.LSig L _) x _ => compile_get_local L x
+    | R.ISetLocal (_, R.LSig L _) x => compile_set_local L x
+    | R.IGetGlobal _ x => compile_get_global x
+    | R.ISetGlobal _ x => compile_set_global x
+    | R.ICoderef _ x => compile_coderef x
+    | R.ICallIndirect (R.Arrow arg_ty _, _) idxs => compile_call_indirect arg_ty idxs
+    | R.ICall (R.Arrow arg_ty _, _) x idxs => compile_call arg_ty x idxs
+    | R.IMemUnpack _ ty _ es => ignore (block_c (translate_arrow_type ty) (forT es compile_instr))
     | R.IStructMalloc _ _ _ =>
         (* TODO: registerroot on the new address;
                  unregisterroot if any field is GC ref being put into GC struct. *)
@@ -543,49 +447,12 @@ Section Instrs.
         (* TODO: unregisterroot fields that may be refs to GC if this struct is MM. *)
         emit (W.BI_call (funcimm me.(me_runtime).(mr_func_free)))
     | R.IStructGet (R.Arrow in_ty _, _) i =>
-        ref <- walloc W.T_i32;;
         fields <- try_option EWrongTypeAnn (head in_ty >>= struct_fields);;
-        field_ty <- try_option EWrongTypeAnn (fst <$> lookup i fields);;
-        offset <- lift_error (struct_field_offset fields i);;
-        emit (W.BI_tee_local (localimm ref));;
-        tagged_load ref (compile_sz offset) field_ty;;
-        val <- save_stack [field_ty];;
-        emit (W.BI_get_local (localimm ref));;
-        let refs := map (fun i => localimm val + i) (find_refs LMNative field_ty) in
-        if_gc_bit_set (W.Tf [] [])
-          (for_gc_ref_vars VSLocal refs
-             (emit (W.BI_call (funcimm me.(me_runtime).(mr_func_registerroot)))))
-          (for_gc_ref_vars VSLocal refs
-             (emit (W.BI_call (funcimm me.(me_runtime).(mr_func_duproot)))));;
-        restore_stack [field_ty] val
+        compile_struct_get fields i
     | R.IStructSet (R.Arrow in_ty _, _) i =>
-        ref <- walloc W.T_i32;;
         fields <- try_option EWrongTypeAnn (head in_ty >>= struct_fields);;
-        field_ty <- try_option EWrongTypeAnn (fst <$> lookup i fields);;
         val_ty <- try_option EWrongTypeAnn (lookup 1 in_ty);;
-        offset <- lift_error (struct_field_offset fields i);;
-
-        emit (W.BI_tee_local (localimm ref));;
-        if_gc_bit_set (W.Tf [] [])
-          (ret tt)
-          (let tys := translate_type field_ty in
-           gc_loads ref (compile_sz offset) tys;;
-           val <- save_stack [field_ty];;
-           let refs := map (fun i => localimm val + i) (find_refs LMNative field_ty) in
-           for_gc_ref_vars VSLocal refs
-             (emit (W.BI_call (funcimm me.(me_runtime).(mr_func_unregisterroot)))));;
-
-        emit (W.BI_get_local (localimm ref));;
-        if_gc_bit_set (W.Tf [] [])
-          (val <- save_stack [val_ty];;
-           let refs := map (fun i => localimm val + i) (find_refs LMNative val_ty) in
-           for_gc_ref_vars VSLocal refs
-             (emit (W.BI_load (memimm me.(me_runtime).(mr_mem_gc)) W.T_i32 None 0%N 0%N));;
-           restore_stack [val_ty] val)
-          (ret tt);;
-
-        emit (W.BI_get_local (localimm ref));;
-        tagged_store' (compile_sz offset) val_ty
+        compile_struct_set fields val_ty i
     | R.IStructSwap _ _ =>
         (* TODO: registerroot if GC struct *)
         raise ETodo
@@ -601,52 +468,9 @@ Section Instrs.
                  duproot a bunch of times if MM array *)
         raise ETodo
     | R.IArrayGet (R.Arrow in_ty _, _) =>
-        (* TODO: registerroot if GC array;
-                 duproot if MM array *)
-        idx <- walloc W.T_i32;;
-        ref <- walloc W.T_i32;;
-        emit (W.BI_set_local (localimm idx));;
-        emit (W.BI_set_local (localimm ref));;
-
-        tagged_load
-          ref
-          (emit (W.BI_const (W.VAL_int32 (Wasm_int.int_of_Z i32m 0))))
-          (R.Num (R.Int R.U R.i32));;
-
-        emit (W.BI_get_local (localimm idx));;
-        emit (W.BI_relop W.T_i32 (W.Relop_i (W.ROI_lt (W.SX_U))));;
-
-        elem_ty <- try_option EWrongTypeAnn (head in_ty >>= array_elem);;
-        let get_offset :=
-          emit (W.BI_get_local (localimm idx));;
-          let words := type_words elem_ty in
-          emit (W.BI_const (W.VAL_int32 (Wasm_int.int_of_Z i32m (Z.of_nat words))));;
-          emit (W.BI_binop W.T_i32 (W.Binop_i W.BOI_mul));;
-          emit (W.BI_const (W.VAL_int32 (Wasm_int.int_of_Z i32m 4)));; (* skip header length word *)
-          emit (W.BI_binop W.T_i32 (W.Binop_i W.BOI_add))
-        in
-        let elem_tys := translate_type elem_ty in
-        if_c (W.Tf [] elem_tys)
-          (tagged_load ref get_offset elem_ty)
-          (emit W.BI_unreachable);;
-        ret tt
+        try_option EWrongTypeAnn (head in_ty >>= array_elem) >>= compile_array_get
     | R.IArraySet (R.Arrow in_ty _, _) =>
-        (* TODO: unregisterroot if GC array;
-                 duproot a bunch of times if MM array *)
-        elem_ty <- try_option EWrongTypeAnn (head in_ty >>= array_elem);;
-        val <- save_stack [elem_ty];;
-        idx <- walloc W.T_i32;;
-        ref <- walloc W.T_i32;;
-        emit (W.BI_set_local (localimm idx));;
-        emit (W.BI_tee_local (localimm ref));;
-        array_bounds_check ref idx;;
-        if_c (W.Tf [] [])
-          (emit (W.BI_get_local (localimm ref));;
-           restore_stack [elem_ty] val;;
-           let words := type_words elem_ty in
-           tagged_store' (array_offset idx words) elem_ty)
-          (emit W.BI_unreachable);;
-        ret tt
+        try_option EWrongTypeAnn (head in_ty >>= array_elem) >>= compile_array_set
     | R.IArrayFree ann =>
         (* TODO: unregisterroot a bunch of times, since this is an MM array *)
         emit (W.BI_call (funcimm me.(me_runtime).(mr_func_free)))
