theories/compiler/codegen.v
@@ -1,0 +1,96 @@
+From Coq Require Import List.
+Import ListNotations.
+Require Import Coq.Program.Basics.
+Local Open Scope program_scope.
+
+From ExtLib.Data.Monads Require Import StateMonad WriterMonad.
+From ExtLib.Structures Require Import Monads.
+Import MonadNotation.
+Local Open Scope monad.
+
+From Wasm Require datatypes.
+
+From RichWasm Require term.
+From RichWasm.compiler Require Import types util.
+Require Import RichWasm.util.dlist.
+Import RichWasm.util.dlist.Notation.
+
+Module R := RichWasm.term.
+Module W := Wasm.datatypes.
+
+Notation wlocal_ctx := (list W.value_type) (only parsing).
+
+Notation dexpr := (dlist W.basic_instruction).
+
+Record codegen (A : Type) :=
+  { uncodegen : stateT wlocal_ctx
+                       (writerT (@DList.Monoid_dlist W.basic_instruction)
+                                (sum error))
+                       A }.
+
+Arguments Build_codegen {A} _.
+Arguments uncodegen {A} _.
+
+Existing Instance Monad_stateT.
+
+Global Instance Monad_codegen : Monad codegen :=
+  { ret := fun _ => Build_codegen ∘ ret;
+    bind := fun _ _ c f => Build_codegen (uncodegen c >>= uncodegen ∘ f) }.
+
+Global Instance MonadExc_codegen : MonadExc error codegen :=
+  { raise := fun _ => Build_codegen ∘ raise;
+    catch := fun _ b h => Build_codegen (catch (uncodegen b) (uncodegen ∘ h)) }.
+
+Global Instance MonadState_codegen : MonadState wlocal_ctx codegen :=
+  { get := Build_codegen get;
+    put := Build_codegen ∘ put }.
+
+Global Instance MonadWriter_codegen : MonadWriter (@DList.Monoid_dlist W.basic_instruction) codegen :=
+  { tell := Build_codegen ∘ tell;
+    listen := fun _ => Build_codegen ∘ listen ∘ uncodegen;
+    (* Work around broken implementation of `pass` in ExtLib.
+       https://github.com/rocq-community/coq-ext-lib/issues/153 *)
+    pass := fun _ c => Build_codegen (mkStateT (fun s =>
+      pass ('(x, f, s) <- runStateT (uncodegen c) s;;
+            ret (x, s, f)))) }.
+
+Definition lift_error {A} (c : error + A) : codegen A :=
+  Build_codegen (lift (lift c)).
+
+Definition try_option {A} (e : error) (x : option A) : codegen A :=
+  match x with
+  | None => raise e
+  | Some x' => ret x'
+  end.
+
+Definition ignore {A} (c : codegen A) : codegen unit :=
+  c;;
+  ret tt.
+
+Definition run_codegen (c : codegen unit) (wl : wlocal_ctx) : error + wlocal_ctx * W.expr :=
+  match runWriterT (runStateT (uncodegen c) wl) with
+  | inl e => inl e
+  | inr x => inr (snd (PPair.pfst x), DList.to_list (PPair.psnd x))
+  end.
+
+Definition emit (e : W.basic_instruction) : codegen unit :=
+  tell (DList.singleton e).
+
+Definition capture {A} (c : codegen A) : codegen (A * dexpr) :=
+  censor (const []%DL) (listen c).
+
+Definition block_c {A} (tf : W.function_type) (c : codegen A) : codegen A :=
+  '(x, es) <- capture c;;
+  emit (W.BI_block tf (DList.to_list es));;
+  ret x.
+
+Definition loop_c {A} (tf : W.function_type) (c : codegen A) : codegen A :=
+  '(x, es) <- capture c;;
+  emit (W.BI_loop tf (DList.to_list es));;
+  ret x.
+
+Definition if_c {A B} (tf : W.function_type) (thn : codegen A) (els : codegen B) : codegen (A * B) :=
+  '(x1, es1) <- capture thn;;
+  '(x2, es2) <- capture els;;
+  emit (W.BI_if tf (DList.to_list es1) (DList.to_list es2));;
+  ret (x1, x2).
